fixed Stub.v
--HG--
branch : adt

platform/cito/Stub.v
@@ -1,104 +1,122 @@
-Require Import CompileFuncSpec.
-
 Set Implicit Arguments.
 
-Require Import Label.
+Require Import ADT.
+Require Import RepInv.
 
-Section TopSection.
+Module Make (Import E : ADT) (Import M : RepInv E).
 
-  Require Import GoodModule.
-  Variable modules : list GoodModule.
-
-  Require Import Semantics.
-  Variable imports : LabelMap.t ForeignFuncSpec.
-
-  Definition FName := SyntaxFunc.Name.
-
-  Definition MName := GoodModule.Name.
-
-  Fixpoint flatten A (ls : list (list A)) :=
-    match ls with
-      | nil => nil
-      | x :: xs => x ++ flatten xs
-    end.
-
-  Require Import GoodFunction.
-  Definition to_internal_func_spec (f : GoodFunction) : InternalFuncSpec :=
-    {|
-      Semantics.Fun := f;
-      Semantics.NoDupArgVars := proj1 (IsGoodFunc f)
-    |}.
-
-  Coercion to_internal_func_spec : GoodFunction >-> InternalFuncSpec.
-
-  Definition exports :=
-    to_map
-      (flatten 
-         (List.map 
-            (fun m =>
-               List.map 
-                 (fun (f : GoodFunction) =>
-                    ((MName m, FName f), f : InternalFuncSpec)
-                 ) (Functions m)
-            ) modules)).
-
-  Definition accessible_labels := keys imports ++ keys exports.
-
-  Section fs.
-
-    Variable stn : settings.
-
-    Require Import ConvertLabel Label.
-    Definition labels (lbl : label) : option W := Labels stn lbl.
-
-    Definition is_label_map_to_word lbl p :=
-      match labels lbl with
-        | Some p' => 
-          if weq p p' then
-            true
-          else
-            false
-        | None => false
-      end.
-
-    Definition is_label_map_to_word' A p (x : label * A) := is_label_map_to_word (fst x) p.
-
-    Definition find_by_word A m (p : W) : option A :=
-      match find (is_label_map_to_word' p) m with
-        | Some (_, a) => Some a
-        | None => None
-      end.
-
-    Definition is_export := find_by_word (LabelMap.elements exports).
-
-    Definition is_import := find_by_word (LabelMap.elements imports).
-
-    Definition fs (p : W) : option Callee :=
-      match is_export p with
-        | Some spec => Some (Internal spec)
-        | None => 
-          match is_import p with
-            | Some spec => Some (Foreign spec)
-            | None => None
-          end
-      end.
-
-  End fs.
-
+  Require Import CompileFuncSpec.
+  Module Import CompileFuncSpecMake := Make E M.
   Require Import Inv.
+  Import InvMake.
+  Require Import Semantics.
+  Import SemanticsMake.
+  Import InvMake2.
 
-  Definition foreign_spec spec : assert := 
-    st ~> ExX, foreign_spec _ spec st.
+  Require Import FMapFacts1.
+  Require Import LabelMap.
+  Module Import BLMF := WFacts_fun LabelKey LabelMap.
+  Require Import Label.
+  Module Import FMapFacts1LabelMapMake := WFacts_fun Key' LabelMap.
 
-  Definition spec_without_funcs_ok_fs (spec : InternalFuncSpec) := spec_without_funcs_ok spec fs.
+  Require Import AutoSep.
+  Require Import StructuredModule.
+  Require Import GoodModule.
+  Require Import GoodFunction.
+  Require Import ConvertLabel.
+  Require Import NameDecoration.
+  Require Import Sumbool.
+  Require Import Wrap.
 
-  Definition bimports_base : list import := 
-    LabelMap.elements 
-      (LabelMap.map foreign_spec imports) ++ 
-    LabelMap.elements 
-      (LabelMap.map spec_without_funcs_ok_fs exports).
-                      
-  Section module.
+  Section TopSection.
+
+    Variable modules : list GoodModule.
+
+    Variable imports : LabelMap.t ForeignFuncSpec.
+
+    Definition FName := SyntaxFunc.Name.
+
+    Definition MName := GoodModule.Name.
+
+    Fixpoint flatten A (ls : list (list A)) :=
+      match ls with
+        | nil => nil
+        | x :: xs => x ++ flatten xs
+      end.
+
+    Definition to_internal_func_spec (f : GoodFunction) : InternalFuncSpec :=
+      {|
+        Semantics.Fun := f;
+        Semantics.NoDupArgVars := proj1 (IsGoodFunc f)
+      |}.
+
+    Coercion to_internal_func_spec : GoodFunction >-> InternalFuncSpec.
+
+    Definition exports :=
+      to_map
+        (flatten 
+           (List.map 
+              (fun m =>
+                 List.map 
+                   (fun (f : GoodFunction) =>
+                      ((MName m, FName f), f : InternalFuncSpec)
+                   ) (Functions m)
+              ) modules)).
+
+    Definition accessible_labels := keys imports ++ keys exports.
+
+    Section fs.
+
+      Variable stn : settings.
+
+      Definition labels (lbl : label) : option W := Labels stn lbl.
+
+      Definition is_label_map_to_word lbl p :=
+        match labels lbl with
+          | Some p' => 
+            if weq p p' then
+              true
+            else
+              false
+          | None => false
+        end.
+
+      Definition is_label_map_to_word' A p (x : label * A) := is_label_map_to_word (fst x) p.
+
+      Definition find_by_word A m (p : W) : option A :=
+        match find (is_label_map_to_word' p) m with
+          | Some (_, a) => Some a
+          | None => None
+        end.
+
+      Definition is_export := find_by_word (LabelMap.elements exports).
+
+      Definition is_import := find_by_word (LabelMap.elements imports).
+
+      Definition fs (p : W) : option Callee :=
+        match is_export p with
+          | Some spec => Some (Internal spec)
+          | None => 
+            match is_import p with
+              | Some spec => Some (Foreign spec)
+              | None => None
+            end
+        end.
+
+    End fs.
+
+    Definition foreign_spec spec : assert := 
+      st ~> ExX, foreign_spec _ spec st.
+
+    Definition spec_without_funcs_ok_fs (spec : InternalFuncSpec) := spec_without_funcs_ok spec fs.
+
+    Definition bimports_base : list import := 
+      LabelMap.elements 
+        (LabelMap.map foreign_spec imports) ++ 
+        LabelMap.elements 
+        (LabelMap.map spec_without_funcs_ok_fs exports).
+    
+    Section module.
 
       Variable m : GoodModule.
 
@@ -114,31 +132,27 @@ Section TopSection.
 
           Definition mod_name := MName m.
 
-          Require Import NameDecoration.
-
           Definition impl_label mod_name f_name : label := (impl_module_name mod_name, f_name).
 
           Definition tgt := impl_label mod_name (FName f).
 
-          Require Import AutoSep.
           Definition body := 
             @Seq_ _ im_g mod_name
-                 (AssertStar_ im mod_name accessible_labels (spec f))
-                 (Goto_ im_g mod_name tgt).
+                  (AssertStar_ im mod_name accessible_labels (CompileFuncSpecMake.spec f))
+                  (Goto_ im_g mod_name tgt).
 
         End body.
 
-        Require Import StructuredModule.
         Definition make_stub : function (GoodModule.Name m) :=
           (FName f, spec_without_funcs_ok f fs, body).
 
       End f.
 
-      Definition Func_to_import (f : GoodFunction) := (impl_label (MName m) (FName f), CompileFuncSpec.spec f).
+      Definition Func_to_import (f : GoodFunction) := (impl_label (MName m) (FName f), CompileFuncSpecMake.spec f).
 
       Definition bimports : list import := 
         bimports_base ++ List.map Func_to_import (Functions m).
-          
+      
       Definition stubs := map make_stub (Functions m).
 
       Definition make_module := StructuredModule.bmodule_ bimports stubs.
@@ -153,11 +167,66 @@ Section TopSection.
              let '(modl, f, pre) := p in
              LabelMap.LabelMap.add (modl, Global f) pre m) imports base.
 
-      Lemma find_importsMap_find_as_map' : 
+      Require Import SetoidList.
+      Require Import GeneralTactics.
+      Lemma InA_eq_List_In : forall elt ls x, InA (@eq elt) x ls <-> List.In x ls.
+        induction ls; simpl; intros.
+        intuition.
+        eapply InA_nil in H; eauto.
+        split; intros.
+        inversion H; subst.
+        eauto.
+        right.
+        eapply IHls.
+        eauto.
+        destruct H.
+        subst.
+        econstructor 1.
+        eauto.
+        econstructor 2.
+        eapply IHls.
+        eauto.
+      Qed.
+
+      Definition equiv_2 A B p1 p2 := forall (a : A) (b : B), p1 a b <-> p2 a b.
+
+      Lemma equiv_2_trans : forall A B a b c, @equiv_2 A B a b -> equiv_2 b c -> equiv_2 a c.
+        unfold equiv_2; intros; split; intros.
+        eapply H0; eapply H; eauto.
+        eapply H; eapply H0; eauto.
+      Qed.
+
+      Lemma eq_key_elt_eq : forall elt, equiv_2 (@LabelMap.eq_key_elt elt) eq.
+        split; intros.
+        unfold LabelMap.eq_key_elt in *.
+        unfold LabelMap.Raw.PX.eqke in *.
+        openhyp.
+        destruct a; destruct b; simpl in *; subst; eauto.
+        subst.
+        unfold LabelMap.eq_key_elt in *.
+        unfold LabelMap.Raw.PX.eqke in *.
+        eauto.
+      Qed.
+
+      Lemma equiv_InA : forall elt (eq1 eq2 : elt -> elt -> Prop), equiv_2 eq1 eq2 -> equiv_2 (InA eq1) (InA eq2).
+        unfold equiv_2; split; intros; eapply InA_weaken; eauto; intros; eapply H; eauto.
+      Qed.
+
+      Lemma InA_eq_key_elt_InA_eq : forall elt, equiv_2 (InA (@LabelMap.eq_key_elt elt)) (InA eq).
+        intros; eapply equiv_InA; eapply eq_key_elt_eq.
+      Qed.
+
+      Lemma InA_eq_key_elt_List_In : forall elt ls x, InA (@LabelMap.eq_key_elt elt) x ls <-> List.In x ls.
+        intros; eapply equiv_2_trans.
+        eapply InA_eq_key_elt_InA_eq.
+        unfold equiv_2; intros; eapply InA_eq_List_In.
+      Qed.
+
+      Lemma find_importsMap_find_list' : 
         forall imps2 imps1 base, 
           NoDupKey (imps1 ++ imps2) -> 
-          (forall (k : label), LabelMap.LabelMap.find (k : Labels.label) base = find_as_map k imps1) ->
-          forall (k : label), LabelMap.LabelMap.find (k : Labels.label) (importsMap' imps2 base) = find_as_map k (imps1 ++ imps2).
+          (forall (k : label), LabelMap.LabelMap.find (k : Labels.label) base = find_list k imps1) ->
+          forall (k : label), LabelMap.LabelMap.find (k : Labels.label) (importsMap' imps2 base) = find_list k (imps1 ++ imps2).
         induction imps2; simpl.
         intros.
         rewrite app_nil_r.
@@ -178,7 +247,7 @@ Section TopSection.
         eauto.
         destruct k0.
         injection e; intros; subst.
-        erewrite In_find_as_map_Some_left.
+        erewrite In_find_list_Some_left.
         eauto.
         eapply NoDup_incl.
         eauto.
@@ -186,11 +255,11 @@ Section TopSection.
         rewrite <- DepList.pf_list_simpl.
         unfold l in *.
         intuition.
-        intuition.
+        eapply InA_eq_key_elt_List_In; intuition.
         unfold LabelKey.eq in *.
-        erewrite add_4.
+        erewrite BLMF.add_4.
         rewrite H0.
-        erewrite find_as_map_neq.
+        erewrite find_list_neq.
         eauto.
         eapply NoDup_incl.
         eauto.
@@ -201,14 +270,14 @@ Section TopSection.
         eauto.
       Qed.
 
-      Lemma find_importsMap_find_as_map : forall imps (k : label), NoDupKey imps -> LabelMap.LabelMap.find (k : Labels.label) (importsMap imps) = find_as_map k imps.
+      Lemma find_importsMap_find_list : forall imps (k : label), NoDupKey imps -> LabelMap.LabelMap.find (k : Labels.label) (importsMap imps) = find_list k imps.
         intros.
         unfold importsMap.
-        erewrite find_importsMap_find_as_map'.
+        erewrite find_importsMap_find_list'.
         erewrite app_nil_l; eauto.
         erewrite app_nil_l; eauto.
         intros.
-        unfold find_as_map.
+        unfold find_list.
         eauto.
       Qed.        
 
@@ -224,8 +293,8 @@ Section TopSection.
         forall mn (fns : list (function mn)) imps impsMap, 
           NoDupKey imps -> 
           incl (map (@func_to_import _) fns) imps -> 
-          (forall (k : label), LabelMap.LabelMap.find (k : Labels.label) impsMap = find_as_map k imps) ->
-          forall (k : label), LabelMap.LabelMap.find (k : Labels.label) (fullImports' impsMap fns) = find_as_map k imps.
+          (forall (k : label), LabelMap.LabelMap.find (k : Labels.label) impsMap = find_list k imps) ->
+          forall (k : label), LabelMap.LabelMap.find (k : Labels.label) (fullImports' impsMap fns) = find_list k imps.
       Proof.
         induction fns; simpl; intros.
         eauto.
@@ -244,32 +313,31 @@ Section TopSection.
         eapply LabelMap.LabelMap.add_1.
         eauto.
         symmetry.
-        eapply In_find_as_map_Some.
+        eapply In_find_list_Some.
         eauto.
         destruct k0.
         injection e; intros; subst.
         unfold func_to_import in *; simpl in *.
-        intuition.
-        erewrite add_4.
+        eapply InA_eq_key_elt_List_In; intuition.
+        erewrite BLMF.add_4.
         eauto.
         eauto.
       Qed.
 
-      Lemma fullImports_no_effect : forall mn (fns : list (function mn)) imps, NoDupKey imps -> incl (map (@func_to_import _) fns) imps -> forall (k : label), LabelMap.LabelMap.find (k : Labels.label) (fullImports imps fns) = find_as_map k imps.
+      Lemma fullImports_no_effect : forall mn (fns : list (function mn)) imps, NoDupKey imps -> incl (map (@func_to_import _) fns) imps -> forall (k : label), LabelMap.LabelMap.find (k : Labels.label) (fullImports imps fns) = find_list k imps.
         intros.
         unfold fullImports.
         specialize fullImports_no_effect'; intros.
         unfold fullImports' in *.
         eapply H1; eauto.
         intros.
-        eapply find_importsMap_find_as_map; eauto.
+        eapply find_importsMap_find_list; eauto.
       Qed.
 
       Lemma incl_stubs_bimports : incl (map (@func_to_import _) stubs) bimports.
         admit.
       Qed.
 
-      Require Import Sumbool.
       Lemma find_spec : forall A f (ls : list A) a, find f ls = Some a -> f a = true /\ In a ls.
         induction ls; simpl; intuition;
         (destruct (sumbool_of_bool (f a)); 
@@ -312,12 +380,14 @@ Section TopSection.
         exists l.
         split.
         eapply In_find_Some; eauto.
-        eauto.
+        eapply InA_eq_key_elt_List_In; intuition.
+        intuition.
         intuition.
         rewrite e0 in H0; intuition.
         rewrite e0 in e; intuition.
         rewrite e in H.
         destruct (is_import stn p); intuition.
+        discriminate.
       Qed.
 
       Lemma augment_elim : 
@@ -352,62 +422,64 @@ Section TopSection.
         eauto.
       Qed.
 
-      Lemma imports_bimports : forall k v, LabelMap.find k imports = Some v -> find_as_map k bimports = Some (foreign_spec v).
+      Lemma imports_bimports : forall k v, LabelMap.find k imports = Some v -> find_list k bimports = Some (foreign_spec v).
         unfold bimports, bimports_base.
         intros.
-        eapply NoDup_app_find_as_map.
+        eapply NoDup_app_find_list.
         eapply NoDup_bimports.
-        eapply NoDup_app_find_as_map.
+        eapply NoDup_app_find_list.
         eapply NoDup_incl.
         eapply NoDup_bimports.
         unfold bimports, bimports_base.
         intuition.
-        rewrite find_as_map_elements.
+        rewrite find_list_elements.
         eapply find_map; eauto.
       Qed.
 
       Corollary in_imports_in_bimports : forall x, LabelMap.In x imports -> In x (map fst bimports).
-        unfold bimports, bimports_base.
-        intros.
-        erewrite map_app.
-        eapply in_or_app.
-        left.
-        erewrite map_app.
-        eapply in_or_app.
-        left.
-        eapply In_In_keys.
-        eapply map_3; eauto.
+      unfold bimports, bimports_base.
+      intros.
+      erewrite map_app.
+      eapply in_or_app.
+      left.
+      erewrite map_app.
+      eapply in_or_app.
+      left.
+      eapply InA_eq_List_In.
+      specialize In_In_keys; intros; unfold keys in *; eapply H0.
+      eapply map_3; eauto.
       Qed.
 
-      Lemma exports_bimports : forall k v, LabelMap.find k exports = Some v -> find_as_map k bimports = Some (spec_without_funcs_ok v fs).
+      Lemma exports_bimports : forall k v, LabelMap.find k exports = Some v -> find_list k bimports = Some (spec_without_funcs_ok v fs).
         unfold bimports, bimports_base.
         intros.
-        eapply NoDup_app_find_as_map.
+        eapply NoDup_app_find_list.
         eapply NoDup_bimports.
-        eapply NoDup_app_find_as_map_2.
+        eapply NoDup_app_find_list_2.
         eapply NoDup_incl.
         eapply NoDup_bimports.
         unfold bimports, bimports_base.
         intuition.
-        rewrite find_as_map_elements.
+        rewrite find_list_elements.
         unfold spec_without_funcs_ok_fs.
         erewrite find_map; eauto.
       Qed.
 
       Corollary in_exports_in_bimports : forall x, LabelMap.In x exports -> In x (map fst bimports).
-        unfold bimports, bimports_base.
-        intros.
-        erewrite map_app.
-        eapply in_or_app.
-        left.
-        erewrite map_app.
-        eapply in_or_app.
-        right.
-        eapply In_In_keys.
-        eapply map_3; eauto.
+      unfold bimports, bimports_base.
+      intros.
+      erewrite map_app.
+      eapply in_or_app.
+      left.
+      erewrite map_app.
+      eapply in_or_app.
+      right.
+      eapply InA_eq_List_In.
+      specialize In_In_keys; intros; unfold keys in *; eapply H0.
+      eapply map_3; eauto.
       Qed.
 
-      Lemma fullImports_eq_bimports : forall (k : label), LabelMap.LabelMap.find (k : Labels.label) (fullImports bimports stubs) = find_as_map k bimports.
+      Lemma fullImports_eq_bimports : forall (k : label), LabelMap.LabelMap.find (k : Labels.label) (fullImports bimports stubs) = find_list k bimports.
         intros.
         eapply fullImports_no_effect.
         eapply NoDup_bimports.
@@ -417,7 +489,9 @@ Section TopSection.
       Corollary bimports_fullImports : forall (x : label), In x (map fst bimports) -> LabelMap.LabelMap.find (x : Labels.label) (fullImports bimports stubs) <> None.
       Proof.
         intros.
-        eapply In_find_as_map_not_None in H.
+        specialize In_find_list_not_None; intros.
+        eapply InA_eq_List_In in H.
+        eapply H0 in H.
         eapply ex_up in H.
         openhyp.
         rewrite fullImports_eq_bimports.
@@ -434,11 +508,15 @@ Section TopSection.
         eapply in_app_or in H.
         destruct H.
 
-        eapply In_In_keys in H.
+        specialize In_In_keys; intros; unfold keys in *.
+        eapply InA_eq_List_In in H.
+        eapply H0 in H.
         eapply in_imports_in_bimports in H.
         eapply bimports_fullImports; eauto.
 
-        eapply In_In_keys in H.
+        specialize In_In_keys; intros; unfold keys in *.
+        eapply InA_eq_List_In in H.
+        eapply H0 in H.
         eapply in_exports_in_bimports in H.
         eapply bimports_fullImports; eauto.
       Qed.
@@ -448,7 +526,9 @@ Section TopSection.
         intros.
         eapply in_or_app.
         right.
-        eapply In_In_keys.
+        specialize In_In_keys; intros; unfold keys in *.
+        eapply InA_eq_List_In.
+        eapply H0.
         eapply In_find_not_None; eauto.
       Qed.
       
@@ -458,21 +538,22 @@ Section TopSection.
         eapply exports_bimports; eauto.
       Qed.
 
-      Lemma tgt_fullImports : forall f, In f (Functions m) -> LabelMap.LabelMap.find (tgt f : Labels.label) (fullImports bimports stubs) = Some (spec f).
+      Lemma tgt_fullImports : forall f, In f (Functions m) -> LabelMap.LabelMap.find (tgt f : Labels.label) (fullImports bimports stubs) = Some (CompileFuncSpecMake.spec f).
         intros.
         rewrite fullImports_eq_bimports. 
         unfold bimports, bimports_base.
-        eapply NoDup_app_find_as_map_2.
+        eapply NoDup_app_find_list_2.
         eapply NoDup_bimports.
         unfold tgt.
         unfold mod_name.
-        eapply In_find_as_map_Some.
+        eapply In_find_list_Some.
         eapply NoDup_incl.
         eapply NoDup_bimports.
         unfold bimports, bimports_base.
         intuition.
         unfold Func_to_import in *; simpl in *.
         eapply in_map with (f := fun x => Func_to_import x) in H.
+        eapply InA_eq_key_elt_List_In.
         eauto.
       Qed.
 
@@ -489,6 +570,7 @@ Section TopSection.
         destruct s.
         rewrite e in H.
         intuition.
+        discriminate.
         rewrite e in H.
         destruct (option_dec (is_import stn p)).
         destruct s.
@@ -514,7 +596,9 @@ Section TopSection.
         exists l.
         split.
         eapply In_find_Some; eauto.
+        eapply InA_eq_key_elt_List_In.
         eauto.
+        intuition.
         intuition.
         rewrite e1 in H0; intuition.
         rewrite e1 in e0; intuition.
@@ -527,7 +611,9 @@ Section TopSection.
         intros.
         eapply in_or_app.
         left.
-        eapply In_In_keys.
+        specialize In_In_keys; intros; unfold keys in *.
+        eapply InA_eq_List_In.
+        eapply H0.
         eapply In_find_not_None; eauto.
       Qed.
       
@@ -589,14 +675,14 @@ Section TopSection.
         rewrite sepFormula_eq; apply Imply_refl.
 
         apply injL; intro.
-        Opaque Inv.foreign_spec.
+        Opaque InvMake2.foreign_spec.
         post; descend.
         instantiate (1 := foreign_spec x0).
         erewrite specs_foreign; eauto.
 
         unfold foreign_spec.
         step auto_ext.
-        Transparent Inv.foreign_spec.
+        Transparent InvMake2.foreign_spec.
         step auto_ext.
         rewrite sepFormula_eq; apply Imply_refl.
       Qed.
@@ -605,7 +691,6 @@ Section TopSection.
 
       Lemma good_vcs : forall ls, (forall x, In x ls -> In x (Functions m)) -> vcs (makeVcs bimports stubs (map make_stub ls)).
         induction ls; simpl; eauto.
-        Require Import Wrap.
         Opaque funcs_ok.
         Opaque spec_without_funcs_ok.
         wrap0.
@@ -625,23 +710,23 @@ Section TopSection.
         eapply good_vcs; eauto.
       Qed.
 
-  End module.
+    End module.
 
-  Definition ms := map make_module modules.
+    Definition ms := map make_module modules.
 
-  Definition empty_module := @StructuredModule.bmodule_ nil "empty_module" nil.
+    Definition empty_module := @StructuredModule.bmodule_ nil "empty_module" nil.
 
-  Fixpoint link_all ls := 
-    match ls with
-      | nil => empty_module
-      | x :: nil => x
-      | x :: xs => link x (link_all xs)
-    end.
+    Fixpoint link_all ls := 
+      match ls with
+        | nil => empty_module
+        | x :: nil => x
+        | x :: xs => link x (link_all xs)
+      end.
 
-  Definition m := link_all ms.
+    Definition m := link_all ms.
 
-  Theorem ok : moduleOk m.
-    admit.
-  Qed.
+    Theorem ok : moduleOk m.
+      admit.
+    Qed.
 
-End TopSection.
+  End TopSection.
